towards fixing sieve

examples/low-level/sieveFun.fst
@@ -1,6 +1,6 @@
 (*--build-config
     variables:LIB=../../lib;
-    other-files:$LIB/ext.fst $LIB/set.fsi $LIB/set.fst $LIB/heap.fst $LIB/st.fst $LIB/list.fst  stack.fst listset.fst
+    other-files:$LIB/ext.fst $LIB/set.fsi $LIB/set.fst $LIB/heap.fst $LIB/st.fst $LIB/all.fst $LIB/list.fst  stack.fst listset.fst
     $LIB/ghost.fst stackAndHeap.fst sst.fst sstCombinators.fst
   --*)
 
@@ -23,6 +23,9 @@ let divides divisor n = ((n % divisor) = 0)*)
 opaque type divides  (divisor :nat) (n:nat) =
 exists (k:nat). k*divisor=n
 
+opaque type nonTrivialDivides  (divisor :nat) (n:nat) =
+divides divisor n /\ divisor < n /\ 1 < divisor
+
 (*this lemma is bogus: divisor could be n*)
 val divisorSmall : n:nat{1<n} -> divisor:nat
   ->
@@ -43,7 +46,8 @@ let divisorSmall n divisor = ()
 
 
 type isNotPrime n =
-exists (d:nat). (1<d /\ d<n /\ (divides d n))
+  exists (d:nat). nonTrivialDivides d n
+
 (*cexists (fun (d:nat) -> (1<d /\ d<n /\ (divides d n)))*)
 
 (*this program has nested loops. first, we define the inner loop*)
@@ -90,17 +94,12 @@ match upto with
 (* in below, markings are done in a reverse order as that of the while loop
 | _ -> markMultiplesUpto n lo (upto-1) (mark n f ((upto-1)*lo))*)
 
-type markedIffMultipleOrInit (n:nat) (lo:nat) (upto:nat{lo*(upto-1)<n})
+type markedIffMultipleOrInit (n:nat) (lo:nat) (upto:nat)
   (init:((k:nat{k<n}) -> Tot bool)) (neww:((k:nat{k<n}) -> Tot bool)) =
-  (forall (k:nat{k < upto}). marked n neww (lo*k))
+  (forall (k:nat{k < upto /\ 1<k /\ lo*k<n}). marked n neww (lo*k))
   /\ (forall (k:nat{k < n}). (marked n init k ==> marked n neww k))
   /\ (forall (k:nat{k < n}). (marked n neww k ==> (marked n init k \/ divides lo k)))
 
-type  innerLoopInv (n:nat) (lo: ref nat)  (li : ref nat) (res:ref ((k:nat{k<n}) -> Tot bool))
-    (initres: ((k:nat{k<n}) -> Tot bool)) (m:smem) =
- distinctRefsExists3 m lo res li
-  /\ ((loopkupRef li m)-1)*(loopkupRef lo m) < n
-  /\ markedIffMultipleOrInit n (loopkupRef lo m) (loopkupRef li m) initres (loopkupRef res m)
 
   (* this works, is totally precise, but is hard to use
   /\ loopkupRef res m = markMultiplesUpto n lov (loopkupRef li m) initres*)
@@ -109,22 +108,21 @@ type  innerLoopInv (n:nat) (lo: ref nat)  (li : ref nat) (res:ref ((k:nat{k<n}) 
             ==> (marked n (loopkupRef res m) ((loopkupRef lo m)*k)))*)
 
 type multiplesMarked2 (n:nat) (bitv : (k:nat{k<n}) -> Tot bool) (lo:nat) =
-(forall (k:nat). (k * lo < n)  ==> marked n bitv (lo*k))
-
+  (forall (k:nat). (k * lo < n /\ 1<k)  ==> marked n bitv (lo*k))
 
 type markedIffDividesOrInit2 (n:nat) (lo:nat)
-  (init:((k:nat{k<n}) -> Tot bool)) (neww:((k:nat{k<n}) -> Tot bool)) =
-  (forall (k:nat{k * lo < n}). marked n neww (lo*k))
-  /\ (forall (k:nat{k < n}). (marked n init k ==> marked n neww k))
-  /\ (forall (k:nat{k < n}). (marked n neww k ==> (marked n init k \/ divides lo k)))
+  (init:((k:nat{k<n}) -> Tot bool)) (newres:((k:nat{k<n}) -> Tot bool)) =
+  (forall (k:nat{k * lo < n /\ 1<k}). marked n newres (lo*k))
+  /\ (forall (k:nat{k < n}). (marked n init k ==> marked n newres k))
+  /\ (forall (k:nat{k < n}). (marked n newres k ==> (marked n init k \/ nonTrivialDivides lo k)))
 
 
 type markedIffDividesOrInit (n:nat) (lo:nat)
    (init:((k:nat{k<n}) -> Tot bool)) (neww:((k:nat{k<n}) -> Tot bool)) =
-    (forall (k:nat{k < n}). (marked n neww k <==> (marked n init k \/ divides lo k)))
+    (forall (k:nat{k < n}). (marked n neww k <==> (marked n init k \/ nonTrivialDivides lo k)))
 
 type multiplesMarked (n:nat) (bitv : (k:nat{k<n}) -> Tot bool) (lo:nat) =
-(forall (m:nat{m<n}). (divides lo m) ==> marked n bitv m)
+  (forall (m:nat{m<n}). (nonTrivialDivides lo m) ==> marked n bitv m)
 
 val multiplesMarkedAsDivides :
   n:nat -> bitv:((k:nat{k<n}) -> Tot bool) -> lo:pos
@@ -132,6 +130,7 @@ val multiplesMarkedAsDivides :
     (requires (multiplesMarked2 n bitv lo))
     (ensures (multiplesMarked n bitv lo))
 let multiplesMarkedAsDivides n bitv lo = ()
+
 
 val multiplesMarkedAsDividesIff :
   n:nat -> initv:((k:nat{k<n}) -> Tot bool) -> newv:((k:nat{k<n}) -> Tot bool) -> lo:pos
@@ -141,18 +140,27 @@ val multiplesMarkedAsDividesIff :
     (*[SMTPatT (markedIffDividesOrInit2 n lo initv newv)]*)
 let multiplesMarkedAsDividesIff n bitv newv lo = (multiplesMarkedAsDivides n newv lo)
 
+
+type  innerLoopInv (n:nat) (lo: ref nat)  (li : ref nat) (res:ref ((k:nat{k<n}) -> Tot bool))
+    (initres: ((k:nat{k<n}) -> Tot bool)) (m:smem) =
+ distinctRefsExists3 m lo res li
+  /\ 1 < (loopkupRef li m)
+  /\ markedIffMultipleOrInit n (loopkupRef lo m) (loopkupRef li m) initres (loopkupRef res m)
+
 val innerLoop : n:nat{n>1}
   -> lo: ref nat
   -> li : ref nat
   -> res : ref ((k:nat{k<n}) -> Tot bool)
   -> initres : ((k:nat{k<n}) -> Tot bool)
   -> Mem unit
-      (requires (fun m ->
+      (requires (fun m -> innerLoopInv n lo li res initres m/\
         (*(refExistsInMem li m) /\ (refExistsInMem lo m) /\ (refExistsInMem res m) /\ (li=!=lo) /\ (lo=!=res) /\ (li=!=res)*)
-        distinctRefsExists3 m lo res li /\ loopkupRef li m = 0
+        loopkupRef li m = 2  /\ 1 < (loopkupRef lo m)
                     /\ loopkupRef res m= initres))
-      (ensures (fun m0 _ m1 -> distinctRefsExists3 m1 lo res li
-                      /\ markedIffDividesOrInit n (loopkupRef lo m1) initres (loopkupRef res m1)
+      (ensures (fun _ _ m -> distinctRefsExists3 m lo res li
+                      /\ (forall (k:nat{k * (loopkupRef lo m) < n /\ 1<k}). marked n (loopkupRef res m) (((loopkupRef lo m))*k))
+                      /\ (forall (k:nat{k < n}). (marked n initres k ==> marked n (loopkupRef res m) k))
+                      /\ (forall (k:nat{k < n}). (marked n (loopkupRef res m) k ==> (marked n initres k \/ divides ((loopkupRef lo m)) k)))
       ))
       (hide (union (singleton (Ref li)) (singleton (Ref res))))
 
@@ -167,7 +175,10 @@ let innerLoop n lo li res initres =
       let lov = memread lo in
       let resv = memread res in
       memwrite li (liv+1);
-      memwrite res (mark n resv (lov * liv))));
+      memwrite res (mark n resv (lov * liv))))
+
+
+
 
     (*the part below has no computaional content; why does SMTPatT not work?*)
       let newv = memread res in
@@ -181,7 +192,6 @@ type distinctRefsExists2
 
 type outerGuardLC (n:nat) (lo : ref nat) (m:smem) =
   (refExistsInMem lo m) && ((loopkupRef lo m) < n)
-
 
 type markedIffHasDivisorSmallerThan (n:nat) (lo:nat)
     (neww:((k:nat{k<n}) -> Tot bool)) =
@@ -234,7 +244,7 @@ let outerLoopBody n lo res u =
   (*pushStackFrame ();*)
   let initres = memread res in
   let lov = memread lo in
-  let li = salloc 0 in
+  let li = salloc 2 in
   let liv = memread li in
   innerLoop n lo li res initres;
   let newres = memread res in
